'embedding_zero' 의 표현 변경 - 내가 원하는 '의미'가 정확히 무엇인지 깨닫게 된다....'형식화'의 위대함...!

src/lean/Nemonuri/Study/StanfordOnline/Compilers/Introduction/_1_2_Compiler.lean
@@ -57,7 +57,23 @@ structure ProduceExecutable (st1 st2: St) : Prop where
 -/
 class ExecutableIsProgram where
   embedding: Function.Embedding (Executable.T St) (Program.T St)
-  another_program (st: St) : embedding (Executable.v st) ≠ (Program.v st)
+  embedding_zero (st: St) : (embedding 0 = 0)
+  another_program (st: St) : (Executable.v st) ≠ 0 → embedding (Executable.v st) ≠ (Program.v st)
+
+/-
+open ExecutableIsProgram Function in
+def ExecutableIsProgram.embedding_zero_iff [ExecutableIsProgram St] (st: St)
+  : (Executable.v st) = 0 ↔ (embedding (Executable.v st) = 0) :=
+  Iff.intro (ExecutableIsProgram.embedding_zero st) (by
+    intro h
+    --have lm1 : Injective (embedding: Embedding (Executable.T St) (Program.T St)) := embedding.injective
+    --unfold Injective at lm1
+    rw [← Injective.eq_iff embedding.injective]
+    rw [h] -- 0 = embedding 0
+    symm
+
+    )
+-/
 
 variable [ExecutableIsProgram St]
 
@@ -80,15 +96,27 @@ export Interpreter (IsRunning IsRunning.isRunning)
 
 variable [IsRunning St]
 
-def isYourProgramRunning (st: St) : Bool := st |> Program.v |> IsRunning.isRunning
+--namespace IsRunning
 
-def isExecutableRunning (st: St) : Bool := st |> Executable.v |> ExecutableIsProgram.embedding |> IsRunning.isRunning
+def IsNonZeroRunning (prog: Program.T St) : Prop := prog ≠ 0 ∧ IsRunning.isRunning prog
 
-def CanBeRunSeparatelyOnData : Prop :=
-  ∃(st: St),
-      (Data.v st ≠ 0) ∧
-      (st |> isYourProgramRunning _ |> not) ∧
-      (st |> isExecutableRunning _)
+--end IsRunning
+
+def IsYourProgramRunning (st: St) : Prop := st |> Program.v |> IsNonZeroRunning _
+
+def IsExecutableRunning (st: St) : Prop := st |> Executable.v |> ExecutableIsProgram.embedding |> IsNonZeroRunning _
+
+structure RunSeparately (data: Data.T St) (st1 st2: St) : Prop where
+  pre: (data ≠ 0) ∧ (Program.v st1 ≠ 0) ∧ (IsExecutableRunning _ st1 |> Not)
+  post: (Data.v st2 = data) ∧
+        (st2 |> IsYourProgramRunning _ |> Not) ∧
+        (st2 |> IsExecutableRunning _)
+/-
+  ∃(st2: St),
+      (Data.v st2 ≠ 0) ∧
+      (st2 |> isYourProgramRunning _ |> not) ∧
+      (st2 |> isExecutableRunning _)
+-/
 
 export Interpreter (Output Output.T Output.v)
 
@@ -96,13 +124,17 @@ variable
   [Output St] [Zero (Output.T St)]
 
 structure WillProduceTheOutput (st1 st2: St) : Prop where
-  pre: (isYourProgramRunning _ st1 |> not) ∧ (isExecutableRunning _ st1) ∧ (Data.v st1 ≠ 0) ∧ (Output.v st1 = 0)
-  post: (isYourProgramRunning _ st2 |> not) ∧ (Output.v st2 ≠ 0)
+  pre: (IsYourProgramRunning _ st1 |> Not) ∧ (IsExecutableRunning _ st1) ∧ (Data.v st1 ≠ 0) ∧ (Output.v st1 = 0)
+  post: (IsYourProgramRunning _ st2 |> Not) ∧ (Output.v st2 ≠ 0)
 
 /-!
 6. And so in this structure the compiler **is offline**, Meaning that we **pre-process** the program first.
 -/
-def IsOffline (st: St) : Prop := (Program.v st ≠ 0) → (Executable.v st = 0) → ¬(isYourProgramRunning _ st)
+structure IsOffline (st1 st2 st3: St) : Prop where
+  pre: (Program.v st1 ≠ 0) ∧ (Executable.v st1 = 0) ∧ (IsExecutableRunning _ st1 |> Not)
+  mid: (Program.v st2 = Program.v st1) ∧ (Executable.v st2 ≠ 0) ∧ (IsExecutableRunning _ st2 |> Not)
+  post: (Program.v st3 = Program.v st2) ∧ (Executable.v st3 = Executable.v st2) ∧ (IsExecutableRunning _ st3)
+
 
 /-!
 7. The compiler is essentially a pre-processing step that produces the executable,
@@ -117,13 +149,24 @@ the program
 -/
 
 def CanRunSameMany {La} (lts: Cslib.LTS St La) : Prop :=
-  ∀(st1: St), (Data.v st1 ≠ 0) ∧ (isExecutableRunning _ st1) →
-  ∀(st2: St), (Data.v st2 ≠ 0) ∧ (isExecutableRunning _ st2) ∧ (Data.v st1 ≠ Data.v st2) →
+  ∀(st1: St), (Data.v st1 ≠ 0) ∧ (IsExecutableRunning _ st1) →
+  ∀(st2: St), (Data.v st2 ≠ 0) ∧ (IsExecutableRunning _ st2) ∧ (Data.v st1 ≠ Data.v st2) →
     (Executable.v st1 = Executable.v st2) →
-  ∃(ls: List La), (lts.MTr st1 ls st2) ∧ (Executable.v st1 = Executable.v st2) ∧
-  ∃(ss: List St), (lts.Execution st1 ls st2 ss) ∧ (ss.Pairwise (fun stL stR => (Data.v stL) = (Data.v stR)))
+  ∃(ls: List La), (Executable.v st1 = Executable.v st2) ∧ (lts.MTr st1 ls st2) ∧
+  ∃(ss: List St), (ss.Pairwise (fun stL stR => (Data.v stL) = (Data.v stR))) ∧ (lts.Execution st1 ls st2 ss)
 
-#print CanRunSameMany
+namespace RunSeparately
+
+protected structure TakeData (data: Data.T St) (st1 st2: St) where
+  pre: (data ≠ 0) ∧ (IsExecutableRunning _ st1 |> Not) ∧ (IsYourProgramRunning _ st1 |> Not)
+  post: (Data.v st2 = data) ∧ (Executable.v st1 = Executable.v st2) ∧ (Program.v st1 = Program.v st2)
+
+@[ext]
+protected structure BeginRun (st1 st2: St) where
+  pre: (Data.v st1 ≠ 0) ∧ (Executable.v st1 ≠ 0) ∧ (IsExecutableRunning _ st1 |> Not)
+  post: (Data.v st2 = Data.v st1) ∧ (IsExecutableRunning _ st1)
+
+end RunSeparately
 
 end spec_s
 
@@ -139,8 +182,57 @@ class State (St: Type us) extends
 
 variable (St: Type us) [State St]
 
+inductive Label where
+  | takeAsInput (prog: Program.T St)
+  | produceExecutable
+  | willProduceTheOutput --InvokeOnTheData
+  | takeData (data: Data.T St)
+  | beginRun
+
+instance instLTS : Cslib.LTS St (Label St) where
+  Tr st1 l st2 :=
+    match l with
+    | .takeAsInput prog => TakeAsInput _ prog st1 st2
+    | .produceExecutable => ProduceExecutable _ st1 st2
+    | .willProduceTheOutput => WillProduceTheOutput _ st1 st2
+    | .takeData data => RunSeparately.TakeData _ data st1 st2
+    | .beginRun => RunSeparately.BeginRun _ st1 st2
+
+#print RunSeparately
+
+--attribute [ext] Cslib.LTS.MTr.split
+
+open Cslib LTS in
+attribute [simp] CanReach IsNonZeroRunning IsYourProgramRunning IsExecutableRunning in
+example (data: Data.T St) (st1 st2: St) (h: RunSeparately _ data st1 st2)
+  : (instLTS _).CanReach st1 st2 := by
+  obtain ⟨h_pre, h_post⟩ := h
+  obtain ⟨h1, h2⟩ := h_pre
+  obtain ⟨h3, h4, h5⟩ := h_post
+  simp at *
+  by_cases h6: Executable.v st1 = 0
+  · have lm1 := (ExecutableIsProgram.embedding_zero _).mp h6
+    simp [lm1] at *
+    clear lm1
+    exists [.takeData data]
+  ·
+/-
+    let w : List (Label St) := [.takeData data, .beginRun]
+    exists w
+    have lm2 : w = ([.takeData data] ++ [.beginRun]) := by subst w ; simp
+    subst w ; rw [lm2]
+    apply (MTr.split_iff (instLTS _)).mpr
+    simp [MTr.single_iff]
+    simp [instLTS]
+    open RunSeparately in
+    constructor
+    · constructor <;> constructor <;> constructor
+      · exact h1
+      · constructor
+-/
 
 
+    --apply (MTr.split_iff (instLTS _)).mpr
 
 
 end def_s
