src/lean/Nemonuri/Study/StanfordOnline/Compilers.lean
@@ -1,1 +1,4 @@
-import Nemonuri.Study.StanfordOnline.Compilers.Introduction
+module
+
+public import Nemonuri.Study.StanfordOnline.Compilers.Lemma
+public import Nemonuri.Study.StanfordOnline.Compilers.Introduction
