src/lean/Nemonuri/Study/StanfordOnline/Compilers/Lemma/Basic.lean
@@ -1,0 +1,30 @@
+module
+
+public import Cslib.Foundations.Semantics.LTS.Basic
+public import Cslib.Foundations.Semantics.LTS.Execution
+
+@[expose] public section public_s
+
+set_option autoImplicit false
+
+variable {State Label : Type*}
+
+
+theorem Cslib.LTS.MTr.single_iff
+  (lts : LTS State Label) (s1 : State) (μ : Label) (s2 : State)
+  : lts.MTr s1 [μ] s2 ↔ lts.Tr s1 μ s2 :=
+  Iff.intro (Cslib.LTS.MTr.single_invert lts s1 μ s2) (Cslib.LTS.MTr.single lts)
+
+
+theorem Cslib.LTS.MTr.split_iff
+  (lts : LTS State Label) {s0 : State} {μs1 μs2 : List Label} {s2 : State}
+  : (lts.MTr s0 (μs1 ++ μs2) s2) ↔ (∃ s1, lts.MTr s0 μs1 s1 ∧ lts.MTr s1 μs2 s2) := by
+  open Cslib LTS Classical in
+  constructor
+  · intro h ; exact MTr.split h
+  · intro h
+    obtain ⟨_, ⟨mtrL, mtrR⟩⟩ := h
+    exact Cslib.LTS.MTr.comp lts mtrL mtrR
+
+
+end public_s
